src/Util/Strings/ParseArithmeticToTaps.v
@@ -1,0 +1,90 @@
+Require Import Coq.Strings.Ascii Coq.Strings.String Coq.Lists.List.
+Require Import Coq.ZArith.ZArith.
+Require Import Crypto.Util.Option.
+Require Import Crypto.Util.OptionList.
+Require Import Crypto.Util.Strings.ParseArithmetic.
+Require Import Crypto.Util.Notations.
+Import ListNotations.
+Local Open Scope option_scope.
+Local Open Scope list_scope.
+Local Open Scope char_scope.
+Local Open Scope string_scope.
+Local Open Scope Z_scope.
+
+Local Open Scope parse_scope.
+
+(** From the Python:
+<<
+# given a string representing one term or "tap" in a prime, returns a pair of
+# integers representing the weight and coefficient of that tap
+#    "2 ^ y" -> [1, y]
+#    "x * 2 ^ y" -> [x, y]
+#    "x * y" -> [x*y,0]
+#    "x" -> [x,0]
+def parse_term(t) :
+    if "*" not in t and "^" not in t:
+        return [int(t),0]
+
+    if "*" in t:
+        if len(t.split("*")) > 2: # this occurs when e.g. [w - x * y] has been turned into [w + -1 * x * y]
+            a1,a2,b = t.split("*")
+            a = int(a1) * int(a2)
+        else:
+            a,b = t.split("*")
+        if "^" not in b:
+            return [int(a) * int(b),0]
+    else:
+        a,b = (1,t)
+
+    b,e = b.split("^")
+    if int(b) != 2:
+        raise NonBase2Exception("Could not parse term, power with base other than 2: %s" %t)
+    return [int(a),int(e)]
+>> *)
+
+(** given an expression representing one term or "tap" in a prime,
+    returns a pair of integers representing the coefficient and weight
+    of that tap:
+    * "2 ^ y" -> Some (2^y, 1)
+    * "x * 2 ^ y" -> Some (2^y, x)
+    * "x * y" -> Some (1,x*y)
+    * "x" -> Some (1,x)
+    *)
+Fixpoint parse_term_of_Zexpr (v : Zexpr) : option (Z * Z)
+  := match v with
+     | Zv x => Some (1, x)
+     | Zopp a => v <- parse_term_of_Zexpr a; Some (fst v, -snd v)
+     | Zadd a b => None
+     | Zsub a b => None
+     | Zmul a b => b <- parse_term_of_Zexpr b; Some (fst b, eval_Zexpr a * snd b)
+     | Zdiv a b => None
+     | Zpow b e => Some (eval_Zexpr v, 1)
+     end%option.
+
+Fixpoint Zexpr_to_add_list (v : Zexpr) : list Zexpr
+  := match v with
+     | Zadd a b => Zexpr_to_add_list a ++ Zexpr_to_add_list b
+     | Zsub a b => Zexpr_to_add_list a ++ [Zopp b]
+     | v => [v]
+     end.
+
+(** Given a Zexpr which is a sequence of additions and subtractions,
+    we return the value of the first component, and a list of the taps
+    for the negation of the other components *)
+Definition parse_prime_and_taps_of_Zexpr (v : Zexpr) : option (Z * list (Z * Z))
+  := match Zexpr_to_add_list v with
+     | nil => None
+     | cons p taps
+       => taps <- Option.List.lift (List.map (fun v => parse_term_of_Zexpr (Zopp v)) taps);
+            Some (eval_Zexpr p, taps)
+     end.
+
+Definition parseZ_arith_to_taps (s : string) : option (Z * list (Z * Z))
+  := v <- parseZexpr_arith s; parse_prime_and_taps_of_Zexpr v.
+
+Local Example parse_v25519 : parse_prime_and_taps_of_Zexpr (2^255 - 19) = Some (2^255, [(1,19)]) := eq_refl.
+Local Example parse_25519 : parseZ_arith_to_taps "2^255 - 19" = Some (2^255, [(1,19)]) := eq_refl.
+Local Example parse_p521 : parseZ_arith_to_taps "2^521 - 1" = Some (2^521, [(1,1)]) := eq_refl.
+Local Example parse_p448 : parseZ_arith_to_taps "2^448 - 2^224 - 1" = Some (2^448, [(2^224,1); (1,1)]) := eq_refl.
+Local Example parse_p256 : parseZ_arith_to_taps "2^256 - 2^224 + 2^192 + 2^96 - 1" = Some (2^256, [(2^224,1); (2^192,-1); (2^96,-1); (1,1)]) := eq_refl.
+Local Example parse_p434 : parseZ_arith_to_taps "2^216 * 3^137 - 1" = Some (2^216 * 3^137, [(1,1)]) := eq_refl.
